Remove assignment forwarding + drop internals passes
They needed to be removed due to assignment forwarding causing
exponential space usage. To make the proof still work I had to make
exact_equivalence and valid_execution look at internal
variables. Intuitively, since we are not dropping them, internal
variables now matter for correctness of Verilog-to-SMT, so we need to
include them in the correctness statements.

- WIP remove separateness requiremens from VerilogToSMT+proof
- WIP continue, just two admits left
- Remove inline/assignment forwarding passes
- WIP Making valid_execution cover internal vars
- WIP trying to reconcile internal/external view of modules for different equivalences
- Remove comments, use ⇓ notation
- DONE!

bin/driver/SMTPP.ml
@@ -16,7 +16,7 @@ module SMTLib = struct
     fprintf fmt "#b%s"
       (String.of_seq
          (List.to_seq
-            (map (function true -> '1' | false -> '0') (List.rev bits))))
+            (List.map (function true -> '1' | false -> '0') (List.rev bits))))
 
   let unaryOp fmt = function
     | BVNot -> fprintf fmt "bvnot"
