vera/VerilogToSMT/VerilogToSMTCorrect.v
@@ -6,6 +6,7 @@ From vera Require Import VerilogSMT.
 From vera Require SMTQueries.
 From vera Require Import VerilogSemantics.
 Import CombinationalOnly.
+Import Facts.
 From vera Require Import Verilog.
 From vera Require Import Bitvector.
 Import RawXBV(bit(..)).
@@ -33,8 +34,8 @@ Import MonadLetNotation.
 Import FunctorNotation.
 Import SigTNotations.
 Local Open Scope monad_scope.
-
 Local Open Scope list.
+Local Open Scope verilog.
 
 Lemma defined_value_for_set_reg_intro_out C regs var xbv :
   (~ C var) ->
@@ -49,55 +50,42 @@ Proof.
   crush.
 Qed.
 
-Lemma module_item_to_smt_satisfiable
-  tag (mi : Verilog.module_item) inputs outputs :
-  disjoint inputs outputs ->
+Lemma module_item_to_smt_satisfiable tag (mi : Verilog.module_item) :
   forall t regs ρ,
-    transfer_module_item tag inputs outputs mi = inr t ->
+    disjoint (Verilog.module_item_reads mi) (Verilog.module_item_writes mi) ->
+    transfer_module_item tag mi = inr t ->
     verilog_smt_match_states_partial
       (fun var => List.In var (Verilog.module_item_reads mi ++ Verilog.module_item_writes mi))
       tag
       (exec_module_item regs mi) ρ ->
     SMTQueries.term_satisfied_by ρ t.
 Proof.
-  funelim (transfer_module_item tag inputs outputs mi); expect 1.
+  funelim (transfer_module_item tag mi); expect 1.
   intros * Hdisjoint * Hexec Hmatch.
   monad_inv; expect 1.
   simp exec_module_item exec_statement in *.
   monad_inv.
   unfold SMTQueries.satisfied_by, SMTQueries.term_satisfied_by. repeat constructor.
   simpl.
-
-  destruct (eval_expr_no_exes _ regs rhs) as [bv_rhs Hbv_rhs]; expect 2. {
-    simp module_item_reads module_item_writes
-      statement_reads statement_writes expr_reads
-      in *.
-    simpl in Hmatch.
-    setoid_rewrite List.in_app_iff in Hmatch .
-    apply verilog_smt_match_states_partial_split_iff in Hmatch.
-    destruct Hmatch as [Hmatch_reads Hmatch_var].
-    eapply defined_value_for_set_reg_intro_out with (var:=var). {
-      rewrite List.Forall_forall in *.
-      eapply disjoint_r_intro in Hdisjoint; eauto.
-    }
-    eapply verilog_smt_match_states_partial_defined_value_for.
-    eassumption.
-  }
-  apply XBV.to_from_bv_inverse in Hbv_rhs. rewrite Hbv_rhs in *.
-
   apply BV.bv_eq_reflect.
 
+  simp module_item_reads module_item_writes
+    statement_reads statement_writes expr_reads
+    in *.
   simpl in Hmatch.
-  simp module_item_reads module_item_writes statement_writes statement_reads expr_reads in Hmatch.
+  disjoint_saturate.
+  unpack_verilog_smt_match_states_partial. 
+  rename_match
+    (verilog_smt_match_states_partial (fun _ => List.In _ (Verilog.expr_reads _)) _ _ _)
+    into Hbefore.
+  rename_match
+    (verilog_smt_match_states_partial (fun _ => List.In _ [var]) _ _ _)
+    into Hafter.
+  apply verilog_smt_match_states_partial_set_reg_out in Hbefore; [|now disjoint_saturate].
   apply XBV.from_bv_injective.
-  erewrite <- Hmatch by eauto with datatypes.
-  rewrite RegisterState.set_reg_get_in.
-  rewrite <- Hbv_rhs.
-  eapply expr_to_smt_value.
-  - eassumption.
-  - unpack_verilog_smt_match_states_partial. 
-    eapply verilog_smt_match_states_partial_set_reg_out; [|eassumption].
-    unfold disjoint in *. rewrite List.Forall_forall in *. firstorder.
+  erewrite <- expr_to_smt_value by eassumption.
+  rewrite <- Hafter by eauto with datatypes.
+  apply RegisterState.set_reg_get_in.
 Qed.
 
 Lemma smt_eq_sat_iff s ρ (l r : SMTLib.term s) :
@@ -108,21 +96,20 @@ Proof.
   simpl. apply SMTLib.value_eqb_eq.
 Qed.
 
-Lemma module_item_to_smt_valid tag  (mi : Verilog.module_item) inputs outputs :
-  disjoint inputs outputs ->
+Lemma module_item_to_smt_valid tag  (mi : Verilog.module_item) :
+  disjoint (Verilog.module_item_reads mi) (Verilog.module_item_writes mi) ->
   forall ρ t,
-    transfer_module_item tag inputs outputs mi = inr t ->
+    transfer_module_item tag mi = inr t ->
     SMTQueries.term_satisfied_by ρ t ->
     forall r1,
       verilog_smt_match_states_partial
         (fun var => List.In var (Verilog.module_item_reads mi))
         tag r1 ρ ->
-          verilog_smt_match_states_partial
-            (fun var => List.In var (Verilog.module_item_reads mi ++ Verilog.module_item_writes mi))
-              tag
-              (exec_module_item r1 mi) ρ.
+      verilog_smt_match_states_partial
+        (fun var => List.In var (Verilog.module_item_writes mi))
+        tag (exec_module_item r1 mi) ρ.
 Proof.
-  funelim (transfer_module_item tag inputs outputs mi);
+  funelim (transfer_module_item tag mi);
     intros * Hdisjoint * Htransf Hsat * Hmatch1; monad_inv; [idtac].
   simp module_item_reads module_item_writes statement_writes statement_reads expr_reads in *.
   simp exec_module_item exec_statement in *.
@@ -131,16 +118,13 @@ Proof.
   pose proof expr_to_smt_valid as Hvalue_match. insterU Hvalue_match.
   inv Hvalue_match. simpl.
   unpack_verilog_smt_match_states_partial.
-  - apply verilog_smt_match_states_partial_set_reg_out; [|assumption].
-    unfold disjoint in *.
-    rewrite List.Forall_forall in *.
-    firstorder.
-  - unfold verilog_smt_match_states_partial.
-    intros. inv H; [|crush].
-    rewrite RegisterState.set_reg_get_in.
-    simpl in Hsat.
-    rewrite Hsat.
-    assumption.
+  all: unfold verilog_smt_match_states_partial.
+  all: intros * [].
+  all: expect 1.
+  rewrite RegisterState.set_reg_get_in.
+  simpl in Hsat.
+  rewrite Hsat.
+  assumption.
 Qed.
 
 Lemma mapT_list_eq_nil A B (f : A -> option B) l :
@@ -157,117 +141,82 @@ Proof.
   some_inv. eauto.
 Qed.
 
-Lemma transfer_module_item_inputs tag inputs outputs mi t :
-  transfer_module_item tag inputs outputs mi = inr t ->
-  list_subset (Verilog.module_item_reads mi) inputs.
+Global Instance verilog_smt_match_states_partial_match_on_proper C :
+  Proper
+    (eq ==> (RegisterState.match_on C) ==> eq ==> iff)
+    (verilog_smt_match_states_partial C).
 Proof.
-  unfold list_subset.
-  funelim (transfer_module_item tag inputs outputs mi); intros; try discriminate.
-  monad_inv.
-  simp module_item_reads statement_reads.
+  repeat intro. subst.
+  unfold verilog_smt_match_states_partial.
+  split.
+  all: intros H var Hvar.
+  all: specialize (H var Hvar).
+  1: rewrite <- H0 by assumption.
+  2: rewrite H0 by assumption.
+  all: assumption.
 Qed.
 
-Lemma transfer_module_item_outputs tag inputs outputs mi t :
-  transfer_module_item tag inputs outputs mi = inr t ->
-  list_subset (Verilog.module_item_writes mi) outputs.
-Proof.
-  unfold list_subset.
-  funelim (transfer_module_item tag inputs outputs mi); intros; try discriminate.
-  monad_inv.
-  simp module_item_writes statement_writes expr_reads.
-  eauto with datatypes.
-Qed.
-
-Lemma transfer_module_body_outputs tag inputs outputs mis t :
-  transfer_module_body tag inputs outputs mis = inr t ->
-  list_subset (Verilog.module_body_writes mis) outputs.
-Proof.
-  funelim (transfer_module_body tag inputs outputs mis); intros; try discriminate.
-  - inv H. simp module_body_writes. constructor.
-  - monad_inv.
-    simp module_body_writes in *.
-    apply list_subset_app.
-    split; eauto using transfer_module_item_outputs with datatypes.
-Qed.
-
-Lemma transfer_module_body_inputs tag inputs outputs mis t :
-  transfer_module_body tag inputs outputs mis = inr t ->
-  list_subset (Verilog.module_body_reads mis) inputs.
-Proof.
-  funelim (transfer_module_body tag inputs inputs mis); intros; try discriminate.
-  - inv H. simp module_body_reads. constructor.
-  - simp transfer_module_body module_body_reads in *.
-    monad_inv.
-    apply list_subset_app.
-    split; eauto using transfer_module_item_inputs with datatypes.
-Qed.
-
-Lemma transfer_module_body_exec_satisfiable inputs outputs body :
+Lemma transfer_module_body_exec_satisfiable inputs body :
   forall tag r1 q ρ,
-    disjoint inputs outputs ->
-    transfer_module_body tag inputs outputs body = inr q ->
+    module_items_sorted inputs body ->
+    transfer_module_body tag body = inr q ->
     verilog_smt_match_states_partial
-      (fun var => List.In var (Verilog.module_body_reads body ++ Verilog.module_body_writes body))
+      (fun var => List.In var (inputs ++ Verilog.module_body_writes body))
       tag (exec_module_body r1 body) ρ ->
     List.Forall (SMTQueries.term_satisfied_by ρ) q.
 Proof.
-  induction body; intros * Hdisjoint Htransfer Hmatch; simp module_body_reads module_body_writes transfer_module_body in *; [some_inv; constructor|].
+  revert inputs.
+  induction body; intros * Hsorted Htransfer Hmatch; simp module_body_reads module_body_writes transfer_module_body in *; [some_inv; constructor|].
   simp exec_module_body in Hmatch. simpl in Hmatch.
   monad_inv.
   constructor.
-  - eapply module_item_to_smt_satisfiable with (inputs := inputs) (regs:=r1).
-    all: try eassumption; expect 1.
-    eapply verilog_smt_match_states_partial_change_regs with (r1 := (exec_module_body (exec_module_item r1 a) body)). {
-      intros.
-      symmetry. eapply Facts.exec_module_body_preserve; [clear H|apply H].
-      unfold disjoint in *.
-      rewrite ! List.Forall_forall in *.
-      setoid_rewrite List.in_app_iff.
-      setoid_rewrite transfer_module_item_inputs; try eassumption.
-      intros var' [Hvar_read|Hvar_write].
-      - setoid_rewrite transfer_module_body_outputs; try eassumption.
-        eauto.
-      - eauto.
-    }
-    eapply verilog_smt_match_states_partial_impl; [|eassumption].
-    intros. simpl.
-    rewrite ! List.in_app_iff in *.
-    intuition assumption.
-  - eapply IHbody; try eauto; [idtac].
+  - inv Hsorted.
+    eapply module_item_to_smt_satisfiable with (regs:=r1); expect 3.
+    { rewrite H1. symmetry. assumption. }
+    { eassumption. }
+    unpack_verilog_smt_match_states_partial.
+    + setoid_rewrite H1.
+      setoid_rewrite <- Facts.exec_module_body_preserve in H; cycle 1.
+      {
+        apply module_items_sorted_no_overwrite in H4.
+	now disjoint_saturate.
+      }
+      assumption.
+    + setoid_rewrite <- Facts.exec_module_body_preserve in H0; cycle 1.
+      {
+        apply module_items_sorted_no_overwrite in H4.
+	now disjoint_saturate.
+      }
+      assumption.
+  - inv Hsorted.
+    eapply IHbody; eauto; expect 1.
     eapply verilog_smt_match_states_partial_impl; [|eassumption].
     intros. simpl.
     rewrite ! List.in_app_iff in *.
     intuition assumption.
 Qed.
 
-Import Facts.
-
-Local Open Scope verilog.
-
 Lemma transfer_module_body_satisfiable v tag ρ q :
-    List.NoDup (Verilog.module_body_writes (Verilog.modBody v)) ->
-    list_subset (Verilog.module_body_reads (Verilog.modBody v)) (Verilog.module_inputs v) ->
-    Permutation (Verilog.module_body_writes (Verilog.modBody v)) (Verilog.module_outputs v) ->
-    disjoint (Verilog.module_inputs v) (Verilog.module_outputs v) ->
+    Permutation (Verilog.modVariables v) (Verilog.module_body_writes (Verilog.modBody v) ++ Verilog.module_inputs v) ->
     module_items_sorted (Verilog.module_inputs v) (Verilog.modBody v) ->
-    transfer_module_body tag (Verilog.module_inputs v) (Verilog.module_outputs v) (Verilog.modBody v) = inr q ->
+    transfer_module_body tag (Verilog.modBody v) = inr q ->
     v ⇓ (execution_of_valuation tag ρ) ->
     List.Forall (SMTQueries.term_satisfied_by ρ) q.
 Proof.
-  intros * Hwrites_ndup Hreads_subset Hwrites_permute Hdisjoint Hsorted Htransfer Hvalid .
+  intros * Hall_driven Hsorted Htransfer Hvalid .
   unfold "⇓" in Hvalid.
   RegisterState.unpack_match_on.
-  rename_match (_ =( Verilog.module_inputs _ )= _) into Hmatch_inputs.
-  rename_match (_ =( Verilog.module_outputs _ )= _) into Hmatch_outputs.
   repeat unfold mk_initial_state, run_vmodule in *.
   rewrite ! sort_module_items_stable in * by eassumption.
   eapply transfer_module_body_exec_satisfiable; eauto.
-  (* apply transfer_module_body_inputs in Htransfer.
-   * rewrite List.Forall_forall in Htransfer. *)
   apply execution_match_on_verilog_smt_match_states_partial.
   RegisterState.unpack_match_on.
-  - setoid_rewrite Hreads_subset. apply Hmatch_inputs.
-  - setoid_rewrite Hwrites_permute. apply Hmatch_outputs.
+  - setoid_rewrite Verilog.module_input_in_vars.
+    apply Hvalid.
+  - setoid_replace (Verilog.module_body_writes (Verilog.modBody v)) with (Verilog.modVariables v)
+      using relation (@list_subset Verilog.variable).
+    2: rewrite Hall_driven; apply list_subset_app_r.
+    apply Hvalid.
 Qed.
 
 Global Instance verilog_smt_match_states_partial_proper C :
@@ -286,75 +235,79 @@ Proof.
     reflexivity.
 Qed.
 
-Lemma transfer_module_body_exec_valid inputs outputs body : forall tag ρ q,
-    disjoint inputs outputs ->
-    list_subset (Verilog.module_body_writes body) outputs ->
-    transfer_module_body tag inputs outputs body = inr q ->
+Lemma transfer_module_body_exec_valid inputs body : forall tag ρ q,
+    module_items_sorted inputs body ->
+    transfer_module_body tag body = inr q ->
     List.Forall (SMTQueries.term_satisfied_by ρ) q ->
     forall r1,
       verilog_smt_match_states_partial
         (fun var => List.In var inputs) tag
 	r1 ρ ->
       verilog_smt_match_states_partial
-        (fun var => List.In var (inputs ++ Verilog.module_body_writes body)) tag
+        (fun var => List.In var (Verilog.module_body_writes body)) tag
 	(exec_module_body r1 body) ρ.
 Proof.
+  revert inputs.
   induction body.
-  all: intros * Hdisjoint Houtputs_in Htransfer Hsat * Hmatch1.
+  all: intros * Hsorted Htransfer Hsat * Hmatch1.
   all: simpl in *.
   all: simp module_body_reads module_body_writes transfer_module_body exec_module_body in *.
   all: autorewrite with list.
   1: crush. all: expect 1.
   unpack_list_subset.
   disjoint_saturate.
-  monad_inv. inv Hsat.
-  rename_match (list_subset (Verilog.module_item_writes a) outputs) into Hitem_writes.
+  monad_inv. inv Hsat. inv Hsorted.
+  rename_match (module_items_sorted (Verilog.module_item_writes a ++ inputs) body) into Hsorted.
   rename_match (list_subset (Verilog.module_item_reads a) inputs) into Hitem_reads.
-  eapply verilog_smt_match_states_partial_split with
-    (C1 := fun var => List.In var (inputs ++ Verilog.module_body_writes body))
-    (C2 := fun var => List.In var (Verilog.module_item_writes a)).
-  - repeat setoid_rewrite List.in_app_iff. intros ? [? | [? | ?]]; auto.
-  - simpl.
-    eapply IHbody; try eassumption; expect 1.
-    setoid_rewrite <- Facts.exec_module_item_preserve; [assumption|].
-    setoid_rewrite Hitem_writes. assumption.
-  - simpl.
-    setoid_rewrite <- Facts.exec_module_body_preserve; [|assumption].
-    eapply verilog_smt_match_states_partial_impl; cycle 1.
-    + eapply module_item_to_smt_valid; cycle 1.
+  simpl.
+  unpack_verilog_smt_match_states_partial.
+  - apply module_items_sorted_no_overwrite in Hsorted. disjoint_saturate.
+    rewrite <- Facts.exec_module_body_preserve by ((symmetry + idtac); assumption).
+    eapply module_item_to_smt_valid.
+    + rewrite Hitem_reads. symmetry. assumption.
+    + eassumption.
+    + eassumption.
+    + setoid_rewrite Hitem_reads. assumption.
+  - eapply IHbody.
+    all: try eassumption.
+    all: expect 1.
+    unpack_verilog_smt_match_states_partial.
+    + eapply module_item_to_smt_valid.
+      * rewrite Hitem_reads. symmetry. assumption.
       * eassumption.
-      * assumption.
+      * eassumption.
       * setoid_rewrite Hitem_reads. assumption.
-      * assumption.
-    + setoid_rewrite List.in_app_iff. auto.
+    + rewrite <- Facts.exec_module_item_preserve
+        by ((symmetry + idtac); assumption).
+      eassumption.
 Qed.
 
 Lemma transfer_module_body_valid tag v ρ q :
   module_items_sorted (Verilog.module_inputs v) (Verilog.modBody v) ->
-  list_subset (Verilog.module_body_reads (Verilog.modBody v)) (Verilog.module_inputs v) ->
-  Permutation (Verilog.module_body_writes (Verilog.modBody v)) (Verilog.module_outputs v) ->
-  List.NoDup (Verilog.module_body_writes (Verilog.modBody v)) ->
-  disjoint (Verilog.module_inputs v) (Verilog.module_outputs v) ->
-  transfer_module_body tag (Verilog.module_inputs v) (Verilog.module_outputs v) (Verilog.modBody v) = inr q ->
+  Permutation (Verilog.modVariables v) (Verilog.module_body_writes (Verilog.modBody v) ++ Verilog.module_inputs v) ->
+  transfer_module_body tag (Verilog.modBody v) = inr q ->
   List.Forall (SMTQueries.term_satisfied_by ρ) q ->
-  valid_execution v (execution_of_valuation tag ρ).
+  v ⇓ execution_of_valuation tag ρ.
 Proof.
-  intros * Hsorted Hinputs_subset Houtputs_permute Hnodup_writes Hdisjoint Htransfer Hsat.
+  intros * Hsorted Hall_driven Htransfer Hsat.
   unfold valid_execution.
   repeat unfold mk_initial_state, run_vmodule in *.
   rewrite sort_module_items_stable by assumption. simpl.
   eapply verilog_smt_match_states_partial_execution_match_on.
-  setoid_rewrite <- Houtputs_permute.
-  eapply transfer_module_body_exec_valid.
-  - eassumption.
-  - rewrite Houtputs_permute. reflexivity.
-  - eassumption.
-  - eassumption.
-  - assert (H : execution_of_valuation tag ρ // Verilog.module_inputs v =( Verilog.module_inputs v )= execution_of_valuation tag ρ). {
-      apply RegisterState.match_on_limit_to_regs_iff.
-      apply RegisterState.limit_to_regs_twice.
-    } rewrite H. clear H.
-    apply verilog_smt_match_states_execution_of_valuation_same.
+  setoid_rewrite Hall_driven.
+  unpack_verilog_smt_match_states_partial.
+  - eapply transfer_module_body_exec_valid.
+    + eassumption.
+    + eassumption.
+    + eassumption.
+    + rewrite RegisterState.limit_to_regs_match_on.
+      apply verilog_smt_match_states_execution_of_valuation_same.
+  - rewrite <- Facts.exec_module_body_preserve.
+    + rewrite RegisterState.limit_to_regs_match_on.
+      apply verilog_smt_match_states_execution_of_valuation_same.
+    + symmetry.
+      eapply module_items_sorted_no_overwrite.
+      apply Hsorted.
 Qed.
 
 Import EqNotations.
@@ -363,60 +316,17 @@ Theorem verilog_to_smt_correct tag v smt :
   verilog_to_smt tag v = inr smt ->
   SMTQueries.smt_reflect
     smt
-    (fun ρ => valid_execution v (execution_of_valuation tag ρ)).
+    (fun ρ => v ⇓ execution_of_valuation tag ρ).
 Proof.
-  intros H ρ.
+  unfold verilog_to_smt.
+  intros Htransf ρ.
+  monad_inv. simpl in *.
   split.
-  - intros Hsat.
-    unfold verilog_to_smt in H.
-    monad_inv. simpl in *.
-    eapply transfer_module_body_valid.
+  all: intros H.
+  - eapply transfer_module_body_valid.
     all: eassumption.
-  - intros Hvalid.
-    unfold verilog_to_smt in H. monad_inv. simpl in *.
-    unfold SMTQueries.satisfied_by. simpl.
-    eapply transfer_module_body_satisfiable.
+  - eapply transfer_module_body_satisfiable.
     all: eassumption.
 Qed.
 
-Lemma defined_value_for_execution_match_on C e' e :
-  e' ={ C }= e ->
-  RegisterState.defined_value_for C e' ->
-  RegisterState.defined_value_for C e.
-Proof.
-  unfold "_ ={ _ }= _", RegisterState.defined_value_for.
-  intros Hmatch Hdefined var HC.
-  insterU Hmatch. insterU Hdefined.
-  destruct Hdefined as [bv ?].
-  exists bv. crush.
-Qed.
-
-(* Move me to semantics *)
-(* Should be replaced by just clean_module *)
-Lemma valid_execution_no_exes_written v : forall e tag q,
-    verilog_to_smt tag v = inr q ->
-    valid_execution v e ->
-    RegisterState.defined_value_for (fun var => List.In var (Verilog.module_inputs v)) e ->
-    RegisterState.defined_value_for (fun var => List.In var (Verilog.module_body_writes (Verilog.modBody v))) e.
-Proof.
-  unfold valid_execution, all_vars_driven.
-  intros * Htransf Hmatch Hinputs_defined.
-  unfold verilog_to_smt in Htransf. monad_inv.
-  rename_match (module_items_sorted _ _) into Hsorted.
-  rename_match (Permutation _ _) into Hout_permute.
-  unfold run_vmodule in Hmatch.
-  rewrite sort_module_items_stable in Hmatch by apply Hsorted.
-  RegisterState.unpack_match_on.
-  rename_match (exec_module_body _ _ =( Verilog.module_outputs _ )= _) into Hmatch_out.
-  setoid_rewrite <- Hout_permute in Hmatch_out.
-  rewrite <- Hmatch_out.
-  apply Clean.exec_module_body_defined with (l_before := Verilog.module_inputs v).
-  - assumption.
-  - apply list_subset_app_r.
-  - unfold mk_initial_state.
-    assert (Hdrop_limit : e // Verilog.module_inputs v =( Verilog.module_inputs v )= e). {
-        apply RegisterState.match_on_limit_to_regs_iff.
-        apply RegisterState.limit_to_regs_twice.
-    } rewrite Hdrop_limit.
-    apply Hinputs_defined.
-Qed.
+Print Assumptions verilog_to_smt_correct.
